starting to work on split, and gave up on proving ToSeq for now, but finished writing it.

examples/MutableBtreeBulkOperations.dfy
@@ -39,11 +39,11 @@ abstract module MutableBtreeBulkOperations {
     }
   }
 
-  method ToSeq(node: Node, keys: array<Key>, values: array<Value>, start: uint64) returns (nextstart: uint64)
+  method ToSeqSubTree(node: Node, keys: array<Key>, values: array<Value>, start: uint64) returns (nextstart: uint64)
     requires WFShape(node)
     requires BS.WF(I(node))
     requires keys.Length == values.Length
-    requires 0 <= start as int < keys.Length
+    requires 0 <= start as int <= keys.Length
     requires start as int + BS.NumElements(I(node)) <= keys.Length
     requires start as int + BS.NumElements(I(node)) < Uint64UpperBound()
     requires keys !in node.repr
@@ -52,8 +52,8 @@ abstract module MutableBtreeBulkOperations {
     ensures nextstart as int == start as int + BS.NumElements(I(node))
     ensures forall i :: 0 <= i < start ==> keys[i] == old(keys[i]);
     ensures forall i :: 0 <= i < start ==> values[i] == old(values[i]);
-    //ensures keys[start..nextstart] == BS.ToSeq(I(node)).0
-    // ensures values[start..nextstart] == BS.ToSeq(I(node)).1
+    ensures keys[start..nextstart] == BS.ToSeq(I(node)).0
+    ensures values[start..nextstart] == BS.ToSeq(I(node)).1
     ensures forall i :: nextstart as int <= i < keys.Length ==> keys[i] == old(keys[i]);
     ensures forall i :: nextstart as int <= i < values.Length ==> values[i] == old(values[i]);
     modifies keys, values
@@ -64,59 +64,77 @@ abstract module MutableBtreeBulkOperations {
       Arrays.Memcpy(values, start, node.contents.values[..node.contents.nkeys]); // FIXME: remove conversion to seq
       nextstart := start + node.contents.nkeys;
     } else {
-      forall i | 0 <= i < node.contents.nchildren
-        ensures BS.NumElementsOfChildren(I(node).children[..i]) <= BS.NumElements(I(node))
-      {
-        BS.NumElementsOfChildrenNotZero(I(node));
-        BS.NumElementsOfChildrenDecreases(I(node).children, i as int);
-      }
+      // forall i | 0 <= i < node.contents.nchildren
+      //   ensures BS.NumElementsOfChildren(I(node).children[..i]) <= BS.NumElements(I(node))
+      // {
+      //   BS.NumElementsOfChildrenNotZero(I(node));
+      //   BS.NumElementsOfChildrenDecreases(I(node).children, i as int);
+      // }
       
       nextstart := start;
-      ghost var inextstart := start as int;
+      // ghost var inextstart := start as int;
       var i: uint64 := 0;
       while i < node.contents.nchildren
-        invariant 0 <= i <= node.contents.nchildren
-        invariant inextstart == start as int + BS.NumElementsOfChildren(I(node).children[..i])
-        invariant inextstart <= keys.Length
-        invariant i < node.contents.nchildren ==> inextstart < keys.Length
-        invariant nextstart as int == inextstart
-        invariant forall i :: 0 <= i < start ==> keys[i] == old(keys[i])
-        invariant forall i :: 0 <= i < start ==> values[i] == old(values[i])
-        //invariant keys[start..nextstart] == BS.Seq.Flatten(BS.ToSeqChildren(I(node).children[..i]).0)
-        // invariant values[start..inextstart] == BS.Seq.Flatten(BS.ToSeqChildren(I(node).children[..i]).1)
-        invariant forall i :: inextstart <= i < keys.Length ==> keys[i] == old(keys[i])
-        invariant forall i :: inextstart <= i < values.Length ==> values[i] == old(values[i])
+      //   invariant 0 <= i <= node.contents.nchildren
+      //   invariant inextstart == start as int + BS.NumElementsOfChildren(I(node).children[..i])
+      //   invariant inextstart <= keys.Length
+      //   invariant i < node.contents.nchildren ==> inextstart < keys.Length
+      //   invariant nextstart as int == inextstart
+      //   invariant forall i :: 0 <= i < start ==> keys[i] == old(keys[i])
+      //   invariant forall i :: 0 <= i < start ==> values[i] == old(values[i])
+      //   //invariant keys[start..nextstart] == BS.Seq.Flatten(BS.ToSeqChildren(I(node).children[..i]).0)
+      //   // invariant values[start..inextstart] == BS.Seq.Flatten(BS.ToSeqChildren(I(node).children[..i]).1)
+      //   invariant forall i :: inextstart <= i < keys.Length ==> keys[i] == old(keys[i])
+      //   invariant forall i :: inextstart <= i < values.Length ==> values[i] == old(values[i])
       {
-        BS.NumElementsOfChildrenNotZero(I(node));
-        BS.NumElementsOfChildrenDecreases(I(node).children, i as int);
-        assert inextstart < keys.Length;
+        //   BS.NumElementsOfChildrenNotZero(I(node));
+        //   BS.NumElementsOfChildrenDecreases(I(node).children, i as int);
+        //   assert inextstart < keys.Length;
         
-        assert I(node).children[..i+1][..i] == I(node).children[..i];
-        inextstart := inextstart + BS.NumElements(I(node).children[i]);
-        BS.NumElementsOfChildrenDecreases(I(node).children, (i + 1) as int);
+        //   assert I(node).children[..i+1][..i] == I(node).children[..i];
+        //   inextstart := inextstart + BS.NumElements(I(node).children[i]);
+        //   BS.NumElementsOfChildrenDecreases(I(node).children, (i + 1) as int);
         
-        ghost var oldnextstart := nextstart;
-        nextstart := ToSeq(node.contents.children[i], keys, values, nextstart);
-
+        //   ghost var oldnextstart := nextstart;
+        assume false;
+        nextstart := ToSeqSubTree(node.contents.children[i], keys, values, nextstart);
         i := i + 1;
 
-        ghost var target := BS.Seq.Flatten(BS.ToSeqChildren(I(node).children[..i]).0);
-        BS.ToSeqChildrenLength(I(node).children[..i]);
-        assert |keys[start..nextstart]| == (nextstart - start) as int;
-        forall j | 0 <= j < (nextstart - start) as int
-          ensures keys[start..nextstart][j] == target[j]
-        {
-          if j < oldnextstart as int {
-            //var oldtarget := BS.Seq.Flatten(BS.ToSeqChildren(I(node).children[..i-1]).0);
-            assume false;
-          } else {
-            assume false;
-          }
-        }
-        assert keys[start..nextstart] == target;
-        assert keys[start..nextstart] == BS.Seq.Flatten(BS.ToSeqChildren(I(node).children[..i]).0);
+        //   ghost var target := BS.Seq.Flatten(BS.ToSeqChildren(I(node).children[..i]).0);
+        //   BS.ToSeqChildrenLength(I(node).children[..i]);
+        //   assert |keys[start..nextstart]| == (nextstart - start) as int;
+        //   forall j | 0 <= j < (nextstart - start) as int
+        //     ensures keys[start..nextstart][j] == target[j]
+        //   {
+        //     if j < oldnextstart as int {
+        //       //var oldtarget := BS.Seq.Flatten(BS.ToSeqChildren(I(node).children[..i-1]).0);
+        //       assume false;
+        //     } else {
+        //       assume false;
+        //     }
+        //   }
+        //   assert keys[start..nextstart] == target;
+        //   assert keys[start..nextstart] == BS.Seq.Flatten(BS.ToSeqChildren(I(node).children[..i]).0);
       }
-      assert I(node).children[..node.contents.nchildren] == I(node).children;
+      // assert I(node).children[..node.contents.nchildren] == I(node).children;
+      assume false;
     }
+  }
+
+  method ToSeq(node: Node) returns (kvlists: (array<Key>, array<Value>))
+    requires WFShape(node)
+    requires BS.WF(I(node))
+    requires BS.NumElements(I(node)) < Uint64UpperBound()
+    ensures (kvlists.0[..], kvlists.1[..]) == BS.ToSeq(I(node))
+    ensures fresh(kvlists.0)
+    ensures fresh(kvlists.1)
+  {
+    var count := NumElements(node);
+    var keys := new Key[count](_ => DefaultKey());
+    var values := new Value[count](_ => DefaultValue());
+    var end := ToSeqSubTree(node, keys, values, 0);
+    assert keys[..] == keys[0..end];
+    assert values[..] == values[0..end];
+    return (keys, values);
   }
 }
